doc

Pycw/Basic.lean
@@ -1,4 +1,3 @@
-import Mathlib.Order.TypeTags
 import Mathlib.Data.Nat.Notation
 import Mathlib.Data.Multiset.AddSub
 import Mathlib.Data.Multiset.Defs
@@ -6,37 +5,55 @@ import Mathlib.Data.Multiset.ZeroCons
 import Mathlib.Data.Finmap
 import Aesop
 
-abbrev Node := WithTop ℕ
-abbrev ω : Node := ⊤
-instance (n : ℕ) : OfNat Node n where
+/-!
+Vertex are numbers & the special one ω. We use Option as the underlying type for convenience.
+-/
+abbrev Vertex := Option ℕ
+instance : DecidableEq Vertex := by unfold Vertex; infer_instance
+abbrev ω : Vertex := none
+instance (n : ℕ) : OfNat Vertex n where
   ofNat := some n
 
+/-!
+An edge is either simple or with a lock. A lock is also represented by a number.
+-/
 abbrev Edge := Option ℕ
-
-instance : DecidableEq Node := by unfold Node WithTop; infer_instance
 instance : DecidableEq Edge := by unfold Edge; infer_instance
 
+/-!
+A chain is a list of vertices and edges interleaved together.
+To avoid reinventing new types, we use two separate lists with
+a hypothesis to ensure the lengths are correct.
+
+Note that we only call it "pre"-chain here, because it is not the real type
+we want to sotre in the map. A real chain has an equivalent relation with its
+inverse, so we need to create a quotient type later, which we will call `Chain`.
+`PreChain` is used for all axiom inputs.
+-/
 structure PreChain where
-  nodes : List Node
+  vertices : List Vertex
   edges : List Edge
-  hlength : nodes.length = edges.length + 1
+  hlength : vertices.length = edges.length + 1
 deriving DecidableEq
 
-lemma PreChain.nodeAtLeast1 (chain : PreChain) : 0 < chain.nodes.length := by
+/-!
+Some utility lemmas and methods for chains
+-/
+lemma PreChain.nodeAtLeast1 (chain : PreChain) : 0 < chain.vertices.length := by
   rw [chain.hlength]
   simp
 
 def PreChain.reverse (chain : PreChain) : PreChain where
-  nodes := chain.nodes.reverse
+  vertices := chain.vertices.reverse
   edges := chain.edges.reverse
   hlength := by simpa using chain.hlength
 
-def PreChain.first (chain : PreChain) : Node :=
-  have : 0 < chain.nodes.length := chain.nodeAtLeast1
-  chain.nodes[0]
+def PreChain.first (chain : PreChain) : Vertex :=
+  have : 0 < chain.vertices.length := chain.nodeAtLeast1
+  chain.vertices[0]
 
-def PreChain.last (chain : PreChain) : Node :=
-  chain.nodes.getLast (by
+def PreChain.last (chain : PreChain) : Vertex :=
+  chain.vertices.getLast (by
     obtain atLeast1 := chain.nodeAtLeast1
     contrapose! atLeast1 with empty
     rw [empty]
@@ -50,13 +67,18 @@ instance (chain : PreChain) : Decidable chain.lockless := by
   unfold PreChain.lockless
   infer_instance
 
+/-!
+Some axioms concerns about subchains, which we define here.
+Note the final version `isSubChain` also allows inverse order,
+which provides convinience for axioms without consulting the quotient type.
+-/
 def PreChain.isSubChainAt (small large : PreChain) (bNodeIndex : ℕ) : Prop :=
   (List.range small.edges.length).attach.Forall (fun i ↦ by
     have : i.val < small.edges.length := by aesop
     exact some small.edges[i.val] = large.edges[bNodeIndex + i.val]?
-  ) ∧ (List.range small.nodes.length).attach.Forall (fun i ↦ by
-    have : i.val < small.nodes.length := by aesop
-    exact some small.nodes[i.val] = large.nodes[bNodeIndex + i.val]?
+  ) ∧ (List.range small.vertices.length).attach.Forall (fun i ↦ by
+    have : i.val < small.vertices.length := by aesop
+    exact some small.vertices[i.val] = large.vertices[bNodeIndex + i.val]?
   )
 
 instance (small large : PreChain) (bNodeIndex : ℕ)
@@ -65,27 +87,30 @@ instance (small large : PreChain) (bNodeIndex : ℕ)
   infer_instance
 
 def PreChain.isSubChain (small large : PreChain) : Prop :=
-  (¬ (List.range large.nodes.length).Forall (fun i ↦ ¬ PreChain.isSubChainAt small large i)) ∨
-  (¬ (List.range large.nodes.length).Forall (fun i ↦ ¬ PreChain.isSubChainAt small.reverse large i))
+  (¬ (List.range large.vertices.length).Forall (fun i ↦ ¬ PreChain.isSubChainAt small large i)) ∨
+  (¬ (List.range large.vertices.length).Forall (fun i ↦ ¬ PreChain.isSubChainAt small.reverse large i))
 
 instance (small large : PreChain)
     : Decidable <| PreChain.isSubChain small large := by
   unfold PreChain.isSubChain
   infer_instance
 
-def PreChain.singleton (node : Node) : PreChain where
-  nodes := [node]
+/-!
+We create methods to construct and update chains, as well as custom notation for them.
+-/
+def PreChain.singleton (vertex : Vertex) : PreChain where
+  vertices := [vertex]
   edges := []
   hlength := by simp
 
-def PreChain.append (chain : PreChain) (edge : Edge) (node : Node) :
+def PreChain.append (chain : PreChain) (edge : Edge) (vertex : Vertex) :
     PreChain where
-  nodes := chain.nodes ++ [node]
+  vertices := chain.vertices ++ [vertex]
   edges := chain.edges ++ [edge]
   hlength := by simpa using chain.hlength
 
 def PreChain.concat (a b : PreChain) (_ : a.last = b.first) : PreChain where
-  nodes := a.nodes ++ b.nodes.eraseIdx 0
+  vertices := a.vertices ++ b.vertices.eraseIdx 0
   edges := a.edges ++ b.edges
   hlength := by
     simp only [List.eraseIdx_zero, List.length_append, List.length_tail]
@@ -94,7 +119,7 @@ def PreChain.concat (a b : PreChain) (_ : a.last = b.first) : PreChain where
 
 def PreChain.setEdge (chain : PreChain) (edgeIndex : ℕ) (edge : Edge) :
     PreChain where
-  nodes := chain.nodes
+  vertices := chain.vertices
   edges := chain.edges.set edgeIndex edge
   hlength := by simpa using chain.hlength
 
@@ -115,6 +140,9 @@ example : ¬ ($4 ~~ 5 ~~ 6).isSubChain ($2 ~L(5)~ 3 ~~ 4 ~~ 5) := by decide
 example : ($1 ~L(3)~ ω ~~ 7).concat ($7 ~~ 5 ~L(0)~ 1) (by decide) = ($1 ~L(3)~ ω ~~ 7 ~~ 5 ~L(0)~ 1) := by decide
 example : ($4 ~~ 5 ~~ 6).setEdge 1 (some 3) = ($4 ~~ 5 ~L(3)~ 6) := by decide
 
+/-!
+We create the real chain type as a quotient.
+-/
 instance PreChainSetoid : Setoid PreChain where
   r := fun a b ↦ a = b ∨ a = b.reverse
   iseqv := {
@@ -139,35 +167,45 @@ instance : Coe PreChain Chain where
 
 example : ($3 ~~ 1 ~L(4)~ ω: Chain) = ($ ω ~L(4)~ 1 ~~ 3: Chain) := by decide
 
+/-!
+An item is a key for multiple times or a key for once.
+-/
 inductive Item
 | Key (lock : ℕ) : Item
 | KeyOnce (lock : ℕ) : Item
 deriving DecidableEq
 
+/-!
+An `ItemMap` assigns keys to vertices. To maintain a normal form,
+we require that the keys are not empty for each entry.
+-/
 abbrev ItemSet := { x : Multiset Item // x ≠ ∅ }
 
-def ItemMap := Finmap (fun (_ : Node) ↦ ItemSet)
+def ItemMap := Finmap (fun (_ : Vertex) ↦ ItemSet)
 deriving DecidableEq
 
 instance : EmptyCollection ItemMap where
   emptyCollection := Finmap.instEmptyCollection.emptyCollection
 
-instance : GetElem ItemMap Node (Multiset Item) (fun _ _ ↦ True) where
+instance : GetElem ItemMap Vertex (Multiset Item) (fun _ _ ↦ True) where
   getElem map i _ := ((map.lookup i).map (·.val)).getD ∅
 
-def ItemMap.set (itemMap : ItemMap) (node : Node) (items : Multiset Item) : ItemMap :=
+def ItemMap.set (itemMap : ItemMap) (vertex : Vertex) (items : Multiset Item) : ItemMap :=
   if h : items ≠ ∅ then
-    itemMap.insert node ⟨items, h⟩
+    itemMap.insert vertex ⟨items, h⟩
   else
-    itemMap.erase node
+    itemMap.erase vertex
 
-def ItemMap.update (itemMap : ItemMap) (node : Node) (updater : Multiset Item → Multiset Item) : ItemMap :=
-  itemMap.set node <| updater <| itemMap[node]
+def ItemMap.update (itemMap : ItemMap) (vertex : Vertex) (updater : Multiset Item → Multiset Item) : ItemMap :=
+  itemMap.set vertex <| updater <| itemMap[vertex]
 
-abbrev im (itemMap : List (Node × (List Item))) : ItemMap :=
+abbrev im (itemMap : List (Vertex × (List Item))) : ItemMap :=
   (itemMap.map (fun entry ↦ (entry.1, (entry.2 : Multiset Item)))).foldl
     (fun itemMap e ↦ itemMap.set e.1 e.2) ∅
 
+/-!
+Also some custom notation for items
+-/
 notation:50 " K(" k:50 ") " => Item.Key k
 notation:50 " K*(" k:50 ") " => Item.KeyOnce k
 example : Multiset Item := [K(2), K*(3), K(2)]
@@ -176,6 +214,9 @@ example : ((im [(4, [K(2), K*(3), K(2)]), (3, [K*(9)])]).set 7 [K(8)]).set 3 ∅
     im [(7, [K(8)]), (5, []), (4, [K(2), K(2), K*(3)])] := by
   decide +native
 
+/-!
+A level is a collection of chains and an item map.
+-/
 structure Level where
   chains : Multiset Chain
   itemMap : ItemMap
@@ -185,4 +226,7 @@ abbrev lv (chains : List PreChain) (itemMap : ItemMap) : Level where
   chains := (chains : List Chain)
   itemMap := itemMap
 
+/-!
+The proposition of "you can win".
+-/
 opaque beatable (level: Level) : Prop
