Pycw/Axiom.lean
@@ -1,19 +1,29 @@
 import Pycw.Basic
 
+/-!
+Base axioms for beatable and unbeatable levels.
+-/
+/-- A level with a single lockless chain from 0 to ω is beatable. -/
 axiom Axiom1 (chain : PreChain) (itemMap : ItemMap)
   (h0 : chain.first = 0) (hω : chain.last = ω) (hlock : chain.lockless) :
   beatable (lv [chain] itemMap)
 
-axiom Axiom2 (a b : PreChain) (itemMap : ItemMap) (hab : a.nodes.inter b.nodes = [])
-  (ha : 0 ∉ a.nodes ∨ ω ∉ a.nodes) (ha : 0 ∉ b.nodes ∨ ω ∉ b.nodes) :
+/-- A level with two disjoint chains with 0 and ω not in the same chain is unbeatable. -/
+axiom Axiom2 (a b : PreChain) (itemMap : ItemMap) (hab : a.vertices.inter b.vertices = [])
+  (ha : 0 ∉ a.vertices ∨ ω ∉ a.vertices) (ha : 0 ∉ b.vertices ∨ ω ∉ b.vertices) :
   ¬ beatable (lv [a, b] itemMap)
 
+/-!
+Rules introduced in chapter one
+-/
+/-- If a level is beatable, one can add an arbitrary chain and it is still beatable. -/
 axiom Rule1_1 (level : Level) (h : beatable level) (chain : PreChain) :
   beatable {
     chains := chain ::ₘ level.chains,
     itemMap := level.itemMap
   }
 
+/-- If a level is beatable, one can remove a subchain and it is still beatable. -/
 axiom Rule1_2 (level : Level) (h : beatable level) (a b : PreChain)
   (hab : a.isSubChain b) (hmem : ([(a : Chain), (b : Chain)] : Multiset Chain) ≤ level.chains) :
   beatable {
@@ -21,6 +31,7 @@ axiom Rule1_2 (level : Level) (h : beatable level) (a b : PreChain)
     itemMap := level.itemMap
   }
 
+/-- If a level is beatable, one can split a chain and it is still beatable. -/
 axiom Rule1_3 (level : Level) (h : beatable level) (a b : PreChain) (hab : a.last = b.first)
   (hmem : ⟦a.concat b hab⟧ ∈ level.chains) :
   beatable {
@@ -28,7 +39,14 @@ axiom Rule1_3 (level : Level) (h : beatable level) (a b : PreChain) (hab : a.las
     itemMap := level.itemMap
   }
 
-
+/-!
+Rules introduced in chapter two
+-/
+/--
+If a level is beatable, one can add lock to an edge
+so long there is a corresponding multi-use key reachable from 0 via another chain,
+and the level is still beatable.
+-/
 axiom Rule2_1 (level : Level) (h : beatable level) (a b : PreChain) (lock : ℕ) (bEdgeIndex : ℕ)
   (ha : a.first = 0) (hkey : Item.Key lock ∈ level.itemMap[a.last])
   (hmem : ([(a : Chain), (b : Chain)] : Multiset Chain) ≤ level.chains)
@@ -39,6 +57,10 @@ axiom Rule2_1 (level : Level) (h : beatable level) (a b : PreChain) (lock : ℕ)
     itemMap := level.itemMap
   }
 
+/--
+If a level is beatable, one can move a single-use key along a lockless chain,
+and the level is still beatable.
+-/
 axiom Rule2_2 (level : Level) (h : beatable level) (chain : PreChain) (key : ℕ)
   (hkey : Item.KeyOnce key ∈ level.itemMap[chain.first])
   (hmem : ⟦chain⟧ ∈ level.chains)
@@ -50,6 +72,10 @@ axiom Rule2_2 (level : Level) (h : beatable level) (chain : PreChain) (key : ℕ
       chain.last ((Item.KeyOnce key) ::ₘ ·)
   }
 
+/--
+If a level is beatable, one can lock a chain and place a reachable single-use key,
+and the level is still beatable.
+-/
 axiom Rule2_3 (level : Level) (h : beatable level) (a b : PreChain) (lock : ℕ)
   (ha : a.first = 0) (hab : a.last = b.first) (hb : b.edges.length = 1)
   (hmem : ([(a : Chain), (b : Chain)] : Multiset Chain) ≤ level.chains) :
@@ -57,13 +83,24 @@ axiom Rule2_3 (level : Level) (h : beatable level) (a b : PreChain) (lock : ℕ)
     chains := (b.setEdge 0 (some lock)) ::ₘ (level.chains.erase b),
     itemMap := level.itemMap.update a.last ((Item.KeyOnce lock) ::ₘ ·)
   }
-axiom Rule3_2 (level : Level) (h : ¬ beatable level) (lock : ℕ) (a b : Node)
+
+/-!
+Rules introduced in chapter three.
+There is no Rule3_1 here because we use Lean's built-in logic for proof by contradiction
+-/
+/--
+If a level is unbeatable, one can lock an edge without a key and it is still unbeatable.
+-/
+axiom Rule3_2 (level : Level) (h : ¬ beatable level) (lock : ℕ) (a b : Vertex)
   (hlock : level.itemMap.all (fun _ items ↦ (Item.Key lock) ∉ items.val ∧ (Item.KeyOnce lock) ∉ items.val)) :
   ¬ beatable {
     chains := ($ a ~L(lock)~ b) ::ₘ level.chains
     itemMap := level.itemMap
   }
 
+/--
+If a level is unbeatable, one can add a useless key reachable from ω, and it is still unbeatable.
+-/
 axiom Rule3_3 (level : Level) (h : ¬ beatable level) (chain : PreChain) (item : Item)
   (hω : chain.last = ω) :
   ¬ beatable {
